code/experimental/poly1305/Hacl.Impl.Poly1305.Field32xN.fst
@@ -590,8 +590,8 @@ let load_felem2_le f b =
   let hi = vec_interleave_high b1 b2 in
   load_felem f lo hi;
   let h1 = ST.get () in
-  vec_interleave_low_lemma64_2 b1 b2;
-  vec_interleave_high_lemma64_2 b1 b2;
+  vec_interleave_low_lemma2 b1 b2;
+  vec_interleave_high_lemma2 b1 b2;
   uints_from_bytes_le_lemma64_2 (as_seq h0 b);
   LSeq.eq_intro (feval h1 f) (S.load_elem2 (as_seq h0 b))
 
@@ -637,15 +637,15 @@ let load_felem4_le f b =
   let hi0 = vec_load_le U128 2 (sub b 32ul 32ul) in
   let lo1 = vec_interleave_low lo0 hi0 in
   let hi1 = vec_interleave_high lo0 hi0 in
-  vec_interleave_low_lemma128_2 lo0 hi0;
-  vec_interleave_high_lemma128_2 lo0 hi0;
+  vec_interleave_low_lemma2 lo0 hi0;
+  vec_interleave_high_lemma2 lo0 hi0;
   let lo2 = cast U64 4 lo1 in
   let hi2 = cast U64 4 hi1 in
 
   let lo = vec_interleave_low lo2 hi2 in
   let hi = vec_interleave_high lo2 hi2 in
-  vec_interleave_low_lemma64_4 lo2 hi2;
-  vec_interleave_high_lemma64_4 lo2 hi2;
+  vec_interleave_low_lemma_uint64_4 lo2 hi2;
+  vec_interleave_high_lemma_uint64_4 lo2 hi2;
 
   load_felem f lo hi;
   let h1 = ST.get () in
@@ -760,7 +760,7 @@ val store_felem2_le:
       as_seq h1 b == BSeq.nat_to_bytes_le 16 ((uint64xN_v hi).[0] * pow2 64 + (uint64xN_v lo).[0]))
 let store_felem2_le b f0 f1 =
   let r0 = vec_interleave_low f0 f1 in
-  vec_interleave_low_lemma64_2 f0 f1;
+  vec_interleave_low_lemma2 f0 f1;
   vec_store_le b r0;
   uints_to_bytes_le_lemma64_2 (vec_v r0)
 
@@ -778,14 +778,14 @@ let store_felem4_le b f0 f1 =
   push_frame ();
   let lo = vec_interleave_low f0 f1 in
   let hi = vec_interleave_high f0 f1 in
-  vec_interleave_low_lemma64_4 f0 f1;
-  vec_interleave_high_lemma64_4 f0 f1;
+  vec_interleave_low_lemma_uint64_4 f0 f1;
+  vec_interleave_high_lemma_uint64_4 f0 f1;
   let lo1 = cast U128 2 lo in
   let hi1 = cast U128 2 hi in
   lemma_cast_vec64_to_vec128 lo;
   lemma_cast_vec64_to_vec128 hi;
   let r0 = vec_interleave_low lo1 hi1 in
-  vec_interleave_low_lemma128_2 lo1 hi1;
+  vec_interleave_low_lemma2 lo1 hi1;
   let tmp = create 32ul (u8 0) in
   vec_store_le tmp r0;
   uints_to_bytes_le_lemma128_2 (vec_v r0);
